src/QUIC.Spec.VarInt.fsti
@@ -3,6 +3,7 @@ module QUIC.Spec.VarInt
 module U62 = QUIC.UInt62
 module U64 = FStar.UInt64
 module LP = LowParse.Spec.BoundedInt // for bounded_int32
+module Cast = FStar.Int.Cast
 
 inline_for_extraction
 let parse_varint_kind = {
@@ -25,3 +26,15 @@ val serialize_bounded_varint
   (min: nat)
   (max: nat { min <= max /\ max < 4294967296 })
 : Tot (LP.serializer (parse_bounded_varint min max))
+
+val varint_len_correct
+  (x: U62.t)
+: Lemma
+  (QUIC.Spec.Base.varint_len x == FStar.Seq.length (LP.serialize serialize_varint x))
+
+val bounded_varint_len_correct
+  (min: nat)
+  (max: nat { min <= max /\ max < 4294967296 })
+  (x: LP.bounded_int32 min max)
+: Lemma
+  (QUIC.Spec.Base.varint_len (Cast.uint32_to_uint64 x) == FStar.Seq.length (LP.serialize (serialize_bounded_varint min max) x))
